solve day 3

problems/3/Problem3.dfy
@@ -1,9 +1,199 @@
+include "../../parser/split.dfy"
+include "../../parser/parseInt.dfy"
+include "../../libraries/src/dafny/Collections/Seqs.dfy"
+include "../../libraries/src/Wrappers.dfy"
 module Problem3 {
+    import opened Split
+    import opened ParseInt
+    import opened Dafny.Collections.Seq
+    import opened Wrappers
+    type Point = (nat, nat)
+    datatype Gear = Gear(val: int, length: nat, pos: Point)
+
+
+
+    method parseInput(input: string) returns (gears: seq<Gear>, symbols: set<Point>)
+    {
+        gears := [];
+        symbols := {};
+        var lines := splitOnBreak(input);
+        for i:nat := 0 to |lines| {
+            var lineGears: seq<Gear> := [];
+            var partialNum: string := "";
+            var numStart: Option<Point> := None;
+            for k:nat := 0 to |lines[i]| {
+                if charInNC(lines[i][k]) && lines[i][k] != '-' {
+                    partialNum := partialNum + [lines[i][k]];
+                    if numStart.None? {
+                        numStart := Some((k,i));
+                    }
+                }else{
+                    if |partialNum| > 0 {
+                        lineGears := lineGears + [Gear(Integer(partialNum), |partialNum|, numStart.UnwrapOr((0,0)))];
+                        partialNum := "";
+                        numStart := None;
+                    }
+                    if lines[i][k] != '.' {
+                        symbols := symbols + {(k,i)};
+                    }
+                }
+            }
+
+            if |partialNum| > 0 {
+                lineGears := lineGears + [Gear(Integer(partialNum), |partialNum|, numStart.UnwrapOr((0,0)))];
+                partialNum := "";
+                numStart := None;
+            }
+            gears := gears + lineGears;
+        }
+    }
+
+    method parseInput2(input: string) returns (gears: seq<Gear>, symbols: set<Point>)
+    {
+        gears := [];
+        symbols := {};
+        var lines := splitOnBreak(input);
+        for i:nat := 0 to |lines| {
+            var lineGears: seq<Gear> := [];
+            var partialNum: string := "";
+            var numStart: Option<Point> := None;
+            for k:nat := 0 to |lines[i]| {
+                if charInNC(lines[i][k]) && lines[i][k] != '-' {
+                    partialNum := partialNum + [lines[i][k]];
+                    if numStart.None? {
+                        numStart := Some((k,i));
+                    }
+                }else{
+                    if |partialNum| > 0 {
+                        lineGears := lineGears + [Gear(Integer(partialNum), |partialNum|, numStart.UnwrapOr((0,0)))];
+                        partialNum := "";
+                        numStart := None;
+                    }
+                    if lines[i][k] == '*' {
+                        symbols := symbols + {(k,i)};
+                    }
+                }
+            }
+
+            if |partialNum| > 0 {
+                lineGears := lineGears + [Gear(Integer(partialNum), |partialNum|, numStart.UnwrapOr((0,0)))];
+                partialNum := "";
+                numStart := None;
+            }
+            gears := gears + lineGears;
+        }
+    }
+
+    function neighborSet(gear: Gear): set<Point> {
+        // set i | gear.pos.1-1 >=0 && 0 < gear.pos.0-1 <= i <= gear.pos.0+gear.length+1 :: (gear.pos.1-1,i)
+        set j,i |  gear.pos.1-1 <= j <= gear.pos.1+1 && 0 <= j &&  gear.pos.0-1 <= i <= gear.pos.0+gear.length && 0 <= i :: (i,j)
+    }
+
+    predicate NextToSymbol(gear: Gear, symbols: set<Point>) {
+        neighborSet(gear) * symbols != {}
+    }
+
     method problem3_1(input: string) returns (x: int) {
-        return 3;
+        var gears, symbols := parseInput(input);
+        // print gears, "\n\n";
+        // print Map(neighborSet, gears), "\n\n";
+        print symbols, "\n\n";
+        var gearmap: map<Point, Gear> := map[];
+        for i := 0 to |gears| {
+            gearmap := gearmap[gears[i].pos := gears[i]];
+        }
+        var nextTo := Filter((gear: Gear) => NextToSymbol(gear, symbols), gears);
+        var notnextTo := Filter((gear: Gear) => !NextToSymbol(gear, symbols), gears);
+        var RL_START_IGNORE := 1 as char;
+        var RL_END_IGNORE := 2 as char;
+        var escape: char := 27 as char;
+        var RED:=[RL_START_IGNORE]+[escape]+"[1;31m"+[RL_END_IGNORE];
+        var BLUE:=[RL_START_IGNORE]+[escape]+"[1;34m"+[RL_END_IGNORE];
+        var GREEN:=[RL_START_IGNORE]+[escape]+"[1;32m"+[RL_END_IGNORE];
+        var NOCOLOR:=[RL_START_IGNORE]+[escape]+"[0m"+[RL_END_IGNORE];
+        // print [RL_START_IGNORE]+[escape]+"[1;31m"+[RL_END_IGNORE];
+        // print notnextTo, "\n";
+        var lines := splitOnBreak(input);
+        var sum := 0;
+        var y :=0;
+        while y < |lines| {
+            var x:=0;
+            while x < |lines[0]| {
+                if (x,y) in symbols {
+                    assume {:axiom} 0 <= x < |lines[y]|;
+                    print BLUE, lines[y][x], NOCOLOR;
+                }else if (x,y) in gearmap.Keys {
+                    if NextToSymbol(gearmap[(x,y)], symbols) {
+                        print GREEN, gearmap[(x,y)].val, NOCOLOR;
+                        sum := sum + gearmap[(x,y)].val;
+                        x := x + gearmap[(x,y)].length-1;
+                    }else{
+                        print RED, gearmap[(x,y)].val, NOCOLOR;
+                        x := x + gearmap[(x,y)].length-1;
+                    }
+                }else{
+                    print ".";
+                }
+                x := x + 1;
+            }
+            print "\n";
+            y := y + 1;
+        }
+        // return FoldLeft((sum: int, gear: Gear) => sum+gear.val, 0, nextTo);
+        return sum;
     }
 
     method problem3_2(input: string) returns (x: int) {
-        return 4;
+        var RL_START_IGNORE := 1 as char;
+        var RL_END_IGNORE := 2 as char;
+        var escape: char := 27 as char;
+        var RED:=[RL_START_IGNORE]+[escape]+"[1;31m"+[RL_END_IGNORE];
+        var BLUE:=[RL_START_IGNORE]+[escape]+"[1;34m"+[RL_END_IGNORE];
+        var GREEN:=[RL_START_IGNORE]+[escape]+"[1;32m"+[RL_END_IGNORE];
+        var NOCOLOR:=[RL_START_IGNORE]+[escape]+"[0m"+[RL_END_IGNORE];
+
+        var gears, symbols := parseInput2(input);
+        var gearmap: map<Point, Gear> := map[];
+        for i := 0 to |gears| {
+            gearmap := gearmap[gears[i].pos := gears[i]];
+        }
+        var lines := splitOnBreak(input);
+        var sum := 0;
+        var y :=0;
+        var pairs: map<Point, seq<Gear>> := map[];
+        while y < |lines| {
+            var x:=0;
+            while x < |lines[0]| {
+                if (x,y) in symbols {
+                    assume {:axiom} 0 <= x < |lines[y]|;
+                    print BLUE, lines[y][x], NOCOLOR;
+                }else if (x,y) in gearmap.Keys {
+                    if NextToSymbol(gearmap[(x,y)], symbols) {
+                        var symbol :| symbol in neighborSet(gearmap[(x,y)]) * symbols;
+                        if symbol in pairs {
+                            pairs := pairs[symbol := pairs[symbol]+[gearmap[(x,y)]]];
+                            assume {:axiom} |pairs[symbol]| == 2;
+                            sum := sum + pairs[symbol][0].val * pairs[symbol][1].val;
+                            // print "sum + ", pairs[symbol][0].val * pairs[symbol][1].val;
+                        }else{
+                            pairs := pairs[symbol := [gearmap[(x,y)]]];
+                        }
+                        print GREEN, gearmap[(x,y)].val, NOCOLOR;
+                        // sum := sum + gearmap[(x,y)].val;
+                        x := x + gearmap[(x,y)].length-1;
+                    }else{
+                        print RED, gearmap[(x,y)].val, NOCOLOR;
+                        x := x + gearmap[(x,y)].length-1;
+                    }
+                }else{
+                    print ".";
+                }
+                x := x + 1;
+            }
+            print "\n";
+            y := y + 1;
+        }
+        // print pairs;
+        return sum;
     }
 }
